WIP type safety SF (logrel_seq)

theories/logrel.v
@@ -60,7 +60,7 @@ Fixpoint safe_lr (Δ : tcontext) (ξ : substitution) (τ : ty) (v : expr) :=
               /\ safe_lr Δ ξ t2 e2
  | Ty_Arrow t1 t2 =>
      exists x e, v = <{ λ x, e }>
-            /\ (forall v', safe_lr Δ ξ t1 v' -> safe_parametrized (safe_lr Δ ξ t2) ( <{[ x / v] e}>))
+            /\ (forall v', safe_lr Δ ξ t1 v' -> safe_parametrized (safe_lr Δ ξ t2) ( <{[ x / v'] e}>))
  | Ty_Forall α t =>
      exists e, v = <{ Λ e }>
             /\ forall (P: expr -> Prop), safe_parametrized (safe_lr (α::Δ) (<[α := P]> ξ) t) e
@@ -132,28 +132,98 @@ Proof.
 Admitted.
 
 (* TODO *)
-Fixpoint logrel_seq Δ Γ ξ (vs : list expr) := True.
+
+Fixpoint logrel_seq_list Δ (lΓ : list (string*ty))  ξ (vs : list expr) : Prop :=
+  match lΓ with
+  | nil => List.length vs = 0
+  | (x,τ)::Γ' =>
+      exists v vs', vs = v::vs'
+               /\ safe_lr Δ ξ τ v
+               /\ logrel_seq_list Δ Γ' ξ vs'
+  end.
+
+Definition logrel_seq Δ Γ ξ (vs : list expr) : Prop :=
+  logrel_seq_list Δ (map_to_list Γ) ξ vs.
+
+Lemma logrel_seq_weaken Δ Γ ξ P vs α :
+not_free_context α Γ ->
+( logrel_seq Δ Γ ξ vs
+ <->
+  logrel_seq (α::Δ) Γ (<[α := P]>ξ) vs
+).
+Proof.
+  intros.
+  split; intros.
+  - generalize dependent Δ.
+    generalize dependent ξ.
+    generalize dependent α.
+    generalize dependent P.
+    generalize dependent vs.
+    induction Γ using map_ind
+    ; intros
+    ; unfold logrel_seq in *.
+    + setoid_rewrite map_to_list_empty in H0.
+      setoid_rewrite map_to_list_empty.
+      by cbn in *.
+    + admit.
+      (* setoid_rewrite map_to_list_insert. *)
+      (* apply IHΓ. *)
+Admitted.
+
 
 Definition context_var Γ : list string :=
   map (fun x => match x with (x1,x2) => x1 end) (gmap_to_list Γ).
 
+Lemma subst_term_seq_insert Γ vs x τ v e :
+  (subst_term_seq (context_var (<[x:=τ]> Γ)) (v :: vs) e) =
+    subst_term x v (subst_term_seq (context_var Γ) (vs) e).
+Admitted.
 Theorem fundamental_theorem Δ Γ τ e :
   Δ;Γ ⊢ e ∈ τ -> (forall ξ vs, logrel_seq Δ Γ ξ vs
-                         -> safe_lr Δ ξ τ (subst_term_seq (context_var Γ) vs e)).
+                         -> safe_parametrized
+                           (safe_lr Δ ξ τ) (subst_term_seq (context_var Γ) vs e)).
 Proof.
-  induction 1; intros; simpl in *.
+  induction 1; intros.
   - (* T_Unit *)
-    split ; auto.
+    apply safe_val; auto.
+    simpl in * ; split ; auto.
   - (* T_Var *)
     admit.
   - (* T_Prod *)
+    rewrite subst_term_seq_pair.
+    repeat intro.
+    pose proof H1 as H1'.
+    apply IHtyping_judgment1 in H1.
+    apply IHtyping_judgment2 in H1'.
+    unfold safe_parametrized in H1,H1'.
     admit.
   - (* T_Fst *)
+    rewrite subst_term_seq_fst; cbn.
+    (* apply IHtyping_judgment in H0. *)
+    (* destruct H0 as (is_val_e & e1 & e2 & is_val_e1 & is_val_e2 & v_pair *)
+    (*                 & Hsafe_e1 & Hsafe_e2). *)
+    (* rewrite v_pair. *)
+    (* backward safe_lr, because fst(e1,e2) -> e1, it suffices to show on e1 *)
     admit.
   - (* T_Snd *)
+    (* rewrite subst_term_seq_snd; cbn in *. *)
+    (* apply IHtyping_judgment in H0. *)
+    (* destruct H0 as (is_val_e & e1 & e2 & is_val_e1 & is_val_e2 & v_pair *)
+    (*                 & Hsafe_e1 & Hsafe_e2). *)
+    (* rewrite v_pair. *)
     admit.
   - (* T_Lam *)
-    admit.
+    rewrite subst_term_seq_lam.
+    apply safe_val;auto.
+    split;auto.
+    exists x. exists (subst_term_seq (context_var Γ) vs e). split; auto.
+    intros.
+    assert ( logrel_seq Δ (<[x := τ1]> Γ) ξ (v'::vs)). admit.
+    apply IHtyping_judgment in H2. simpl in H2.
+    cbn in H2.
+    unfold subst_term_seq in H2.
+    rewrite subst_term_seq_insert in H2.
+    apply H2.
   - (* T_App *)
     admit.
   - (* T_TLam *)
