theories/syntax_systemF.v
@@ -177,6 +177,42 @@ Fixpoint subst_term_seq (xs : list string) (vs : list expr) (t : expr) : expr :=
   | <{ Λ t1 }> => <{ Λ (subst_term_seq xs vs t1) }>
   end.
 
+(* Lemma subst_term_seq_pair xs vs e1 e2 : *)
+(*   subst_term_seq xs vs <{⟨e1, e2⟩}> = *)
+(*   expr_pair (subst_term_seq xs vs e1) (subst_term_seq xs vs e2). *)
+(* Proof. *)
+(*   by simpl. *)
+(* Qed. *)
+
+(* Lemma subst_term_seq_fst xs vs e : *)
+(*   subst_term_seq xs vs <{fst e}> = *)
+(*   expr_fst (subst_term_seq xs vs e). *)
+(* Proof. *)
+(*   by simpl. *)
+(* Qed. *)
+
+(* Lemma subst_term_seq_snd xs vs e : *)
+(*   subst_term_seq xs vs <{snd e}> = *)
+(*   expr_snd (subst_term_seq xs vs e). *)
+(* Proof. *)
+(*   by simpl. *)
+(* Qed. *)
+
+(* Lemma subst_term_seq_lam xs vs x e : *)
+(*   (* TODO miss a condition: x ∉ xs *) *)
+(*   subst_term_seq xs vs <{ λ x, e }> = *)
+(*   expr_abs x (subst_term_seq xs vs e). *)
+(* Proof. *)
+(* Admitted. *)
+
+(* Lemma subst_term_seq_app xs vs e1 e2 : *)
+(*   subst_term_seq xs vs <{e1 e2}> = *)
+(*   expr_app (subst_term_seq xs vs e1) (subst_term_seq xs vs e2). *)
+(* Proof. *)
+(*   by simpl. *)
+(* Qed. *)
+
+
 Definition context := gmap string ty.
 Definition tcontext := list string.
 
@@ -206,10 +242,8 @@ Inductive appears_free_in (x : string) : expr → Prop :=
 
 Inductive free (α : string) : ty -> Prop :=
 | free_var : free α (Ty_Var α)
-| free_pair1 : forall τ1 τ2, free α τ1 -> free α <{ τ1 × τ2 }>
-| free_pair2 : forall τ1 τ2, free α τ2 -> free α <{ τ1 × τ2 }>
-| free_arrow1 : forall τ1 τ2, free α τ1 -> free α <{ τ1 -> τ2 }>
-| free_arrow2 : forall τ1 τ2, free α τ2 -> free α <{ τ1 -> τ2 }>
+| free_pair : forall τ1 τ2, free α τ1 -> free α τ2 -> free α <{ τ1 × τ2 }>
+| free_arrow : forall τ1 τ2, free α τ1 -> free α τ2  -> free α <{ τ1 -> τ2 }>
 | free_forall : forall τ β, α ≠ β -> free α τ -> free α <{ ∀ β, τ }>.
 
 Definition not_free α (Γ : context) (t : string * ty) : Prop :=
